VC/Verif_kalloc.v
@@ -1,3 +1,98 @@
+(** * Verif_kalloc: Memory Allocation ADT implemented by linked lists *)
+
+(** Here is a little C program, [kalloc.c]
+
+    #include "types.h"
+    #include "param.h"
+    #include "memlayout.h"
+    #include "spinlock.h"
+    #include "riscv.h"
+    #include "defs.h"
+
+    void freerange(void *pa_start, void *pa_end);
+
+    extern char end[]; // first address after kernel.
+                      // defined by kernel.ld.
+
+    struct run {
+      struct run *next; 
+    };
+
+    struct {
+      struct spinlock lock;
+      struct run *freelist;
+    } kmem;
+
+    void
+    kinit()
+    {
+      initlock(&kmem.lock, "kmem");
+      freerange(end, (void* )PHYSTOP);
+    }
+
+    void
+    freerange(void *pa_start, void *pa_end)
+    {
+      char *p;
+      p = (char* )PGROUNDUP((uint64)pa_start);
+      for(; p + PGSIZE <= (char* )pa_end; p += PGSIZE)
+        kfree(p);
+    }
+
+    // Free the page of physical memory pointed at by pa,
+    // which normally should have been returned by a
+    // call to kalloc().  (The exception is when
+    // initializing the allocator; see kinit above.)
+    void
+    kfree(void *pa) // LINE: kind of add ( push)
+    {
+      struct run *r;
+
+      if(((uint64)pa % PGSIZE) != 0 || (char* )pa < end || (uint64)pa >= PHYSTOP)
+        panic("kfree");
+
+      // Fill with junk to catch dangling refs.
+      memset(pa, 1, PGSIZE);
+
+      r = (struct run* )pa;
+
+      acquire(&kmem.lock);
+      r->next = kmem.freelist;
+      kmem.freelist = r;
+      release(&kmem.lock);
+    }
+
+    // Allocate one 4096-byte page of physical memory.
+    // Returns a pointer that the kernel can use.
+    // Returns 0 if the memory cannot be allocated.
+    void *
+    kalloc(void) // LINE: kind of remove / pop
+    {
+      struct run *r;
+
+      acquire(&kmem.lock);
+      r = kmem.freelist;
+      if(r)
+        kmem.freelist = r->next;
+      release(&kmem.lock);
+
+      if(r)
+        memset((char* )r, 5, PGSIZE); // fill with junk
+      return (void* )r;
+    }
+
+    This program implements a physical memory allocator, for user processes,
+    kernel stacks, page-table pages,and pipe buffers. Allocates whole 4096-byte pages.
+    - To create a new linked list of free pages
+    - To free up pages (add pages to the linked list)
+    - To allocate pages (pop pages from the linked list)
+
+    This memory allocator is implemented as a header node ([struct run])
+    pointing to a linked list of next cells ([struct next]). *)
+
+(* ================================================================= *)
+(** ** Let's verify! *)
+
 Require VC.Preface. (* Check for the right version of VST *)
 Require Import VST.floyd.proofauto.
 Require Import VST.floyd.library.
@@ -5,3 +100,274 @@ Require Import VC.kalloc.
 #[export] Instance CompSpecs : compspecs. make_compspecs prog. Defined.
 Definition Vprog : varspecs.  mk_varspecs prog. Defined.
 Require Import VC.hints.  (* Import special hints for this tutorial. *)
+
+
+
+
+(*  
+    - Functional model (often in the form of a Coq function)
+    - API specification
+    - Function-body correctness proofs, one per file. 
+*)
+
+(* Functional model *)
+(* Define the type of memory addresses *)
+Definition addr := nat.
+
+(* Define a structure to represent a 'run' as a linked list *)
+Inductive run :=
+  | Run : addr -> option run -> run.
+
+(* Define a structure to represent the memory allocator state *)
+Record kmem := {
+  lock : bool;            (* Indicates whether the lock is acquired or not *)
+  freelist : option run;  (* Pointer to the free list of memory blocks *)
+}.
+
+(*Definition lock : base.val :=
+  λ: "l", repeat (CAS "l" unlocked locked).
+*)
+(*Definition isLock (l : loc) J : vPred :=
+  ((Rel l (Q J) Q_dup)
+  ∗ (RMWAcq l (Q J) Q_dup)
+  ∗ (Init l)
+  ).
+*)
+
+
+(* Lock acquisition function *)
+Definition acquire (kmem : kmem) :=
+  {| lock := true; freelist := kmem.(freelist) |}.
+
+(* Lock release function *)
+Definition release (kmem : kmem) :=
+  {| lock := false; freelist := kmem.(freelist) |}.
+
+(* Free a page of memory, ensuring locking discipline *)
+Definition kfree (kmem : kmem) (p : addr) :=
+  (* Create a new run node for the freed page.
+    - `p` is the address of the freed page.
+    - `kmem.(freelist)` is the current free list (possibly empty).
+    - This effectively pushes `p` onto the free list. *)
+  let new_run := Run p kmem.(freelist) in
+  (* Return a new kmem record with:
+      - The same lock state.
+      - An updated freelist with `new_run` at the head. *)
+  {| lock := kmem.(lock); freelist := Some new_run |}.
+
+(* Safe kfree: Ensures the lock is held before modifying *)
+Definition safe_kfree (kmem : kmem) (p : addr) :=
+  let kmem_locked := acquire kmem in  (* Acquire lock *)
+  let kmem_freed := kfree kmem_locked p in (* Perform free *)
+  release kmem_freed.  (* Release lock *)
+
+(* Allocate a page, ensuring locking discipline *)
+Definition kalloc (kmem : kmem) :=
+  let kmem_locked := acquire kmem in (* Acquire lock *)
+  match kmem_locked.(freelist) with
+  | None => (None, release kmem_locked) (* No available memory *)
+  | Some (Run p next) =>
+      (Some p, release {| lock := kmem_locked.(lock); freelist := next |}) (* Allocate *)
+  end.
+
+
+
+
+
+(* Free a page of memory, add it to the freelist *)
+(*Definition kfree (kmem : kmem) (p : addr) :=
+
+  let new_run := Run p kmem.(freelist) in
+  
+  {| lock := kmem.(lock); freelist := Some new_run |}.*)
+
+
+
+
+
+(* Inductive definition of linked lists (the freelist) *)
+Definition t_list := Tstruct _run noattr.
+
+
+
+(* Representation of the list and lemmas *)
+Fixpoint listrep (sigma: list val) (p: val) : mpred :=
+ match sigma with
+ | h::hs =>
+    EX y:val,  
+        data_at Tsh t_list (y) p * listrep hs y
+ | nil =>
+    !! (p = nullval) && emp
+ end.
+
+Arguments listrep sigma p : simpl never.
+
+
+Lemma listrep_local_facts:
+  forall sigma p,
+   listrep sigma p |--
+   !! (is_pointer_or_null p /\ (p=nullval <-> sigma=nil)).
+Proof.
+intros.
+revert p; induction sigma; intros p; unfold listrep.
+- entailer!. split; auto.
+- fold listrep. Intros y. entailer!.
+ split; intro.
+ + subst p; eapply field_compatible_nullval; eauto.
+ + inversion H2.
+Qed.
+
+(** Now we add this lemma to the Hint database called [saturate_local] *)
+#[export] Hint Resolve listrep_local_facts : saturate_local.
+
+
+Lemma listrep_valid_pointer:
+  forall sigma p,
+   listrep sigma p |-- valid_pointer p.
+Proof.
+ intros.
+ unfold listrep.
+ destruct sigma; simpl.
+- entailer!.
+- Intros y.
+  auto with valid_pointer.
+Qed.
+
+#[export] Hint Resolve listrep_valid_pointer : valid_pointer.
+
+(* Functional Model *)
+
+Definition trun := Tstruct _run noattr.
+Definition tkmem := Tstruct _kmem noattr.
+
+Fixpoint freelistrep (il: list val) (p: val) : mpred :=
+  match il with
+  | h::t =>
+      EX next: val,
+      data_at Ews (trun) next p * 
+      freelistrep t next
+  | nil => !! (p = nullval) && emp
+  end.
+(*
+Definition kmemrep (il : list val) (p: val) : mpred :=
+  EX bl: list (list byte * Z),
+  !! (contents = map fst bl) &&
+  malloc_token Ews thashtable p * 
+  data_at Ews thashtable (map snd bl) p 
+  * iter_sepcon (uncurry listrep) bl.
+
+Definition hashtable_rep (contents: hashtable_contents) (p: val) : mpred :=
+  EX bl: list (list (list byte * Z) * val),
+    !! (contents = map fst bl) &&
+    malloc_token Ews thashtable p * 
+    data_at Ews thashtable (map snd bl) p 
+    * iter_sepcon (uncurry listrep) bl.
+
+
+Definition list_cell (key: list byte) (count: Z) (next: val) (p: val): mpred :=
+ EX kp: val, cstring Ews key kp 
+             * malloc_token Ews (tarray tschar (Zlength key + 1)) kp
+             * data_at Ews tcell (kp,(Vint (Int.repr count), next)) p 
+             * malloc_token Ews tcell p.
+
+
+
+
+Definition spinlock_inv lock_ptr := 
+  EX locked: val, 
+    data_at Ews (Tstruct _spinlock noattr) locked lock_ptr.
+
+Definition kmemrep (il: list val) (p: val) :=
+  EX lock_ptr: val, EX freelist_ptr: val,
+    malloc_token Ews (Tstruct _kmem noattr) p * 
+    data_at Ews (Tstruct _kmem noattr) (lock_ptr, freelist_ptr) p *
+    spinlock_inv lock_ptr *
+    freelistrep il freelist_ptr.
+  
+
+
+Definition stack (il: list val) (p: val) :=
+  EX q:val,
+    malloc_token Ews (Tstruct _kmem noattr) p * 
+    data_at Ews (Tstruct _kmem noattr)  *
+    freelistrep il q.
+
+Definition kmemrep (il: list val) (kmem_ptr: val) : mpred :=
+  
+  EX freelist: val,
+    malloc_token Ews (Tstruct _kmem noattr) kmem_ptr *
+    data_at Ews (Tstruct _kmem noattr) (struct_tuple [default_val (Tstruct _spinlock noattr); freelist]) kmem_ptr *
+    freelistrep il freelist.
+
+
+
+
+  Definition kmemrep (il: list val) (kmem_ptr: val) : mpred :=
+    EX freelist: val,
+      data_at Ews (Tstruct _kmem noattr) (default_val (Tstruct _spinlock noattr), freelist) kmem_ptr * 
+      freelistrep il freelist.
+
+Definition kmemrep (il: list val) (kmem_ptr: val) : mpred :=
+  EX freelist: val,
+    data_at Ews (Tstruct _run noattr) freelist kmem_ptr * 
+    freelistrep il freelist.
+  
+
+(* API specification *)
+
+    (* Specification of freelist *)
+Check data_at.
+(*
+Definition freelist (il : list Z) (p : val)
+
+Definition kfree_spec : ident * funspec :=
+ DECLARE _kfree
+ WITH t: type, p:val, gv: globals
+ PRE [ tptr tvoid ]
+     PROP ()
+     PARAMS (p)
+     SEP (mem_mgr gv; malloc_token Ews t p; data_at_ Ews t p)
+ POST [ Tvoid ]
+     PROP () RETURN () SEP (mem_mgr gv).
+
+
+
+
+Definition reverse_spec : ident * funspec :=
+ DECLARE _kfree
+  WITH sigma : list val, p: val
+  PRE  [ tptr t_list ]
+     PROP ()  PARAMS (p)  SEP (listrep sigma p)
+  POST [ (tptr t_list) ]
+    EX q:val,
+     PROP ()  RETURN (q)  SEP (listrep(rev sigma) q).
+
+
+Definition malloc_spec_example  :=
+ DECLARE _malloc
+ WITH t:type, gv: globals
+ PRE [ tuint ]
+    PROP (0 <= sizeof t <= Int.max_unsigned;
+          complete_legal_cosu_type t = true;
+          natural_aligned natural_alignment t = true)
+    PARAMS (Vint (Int.repr (sizeof t)))
+    SEP (mem_mgr gv)
+ POST [ tptr tvoid ] EX p:_,
+    PROP ()
+    RETURN (p)
+    SEP (mem_mgr gv;
+            if eq_dec p nullval then emp
+            else (malloc_token Ews t p * data_at_ Ews t p)).
+
+Definition free_spec_example :=
+ DECLARE _free
+ WITH t: type, p:val, gv: globals
+ PRE [ tptr tvoid ]
+     PROP ()
+     PARAMS (p)
+     SEP (mem_mgr gv; malloc_token Ews t p; data_at_ Ews t p)
+ POST [ Tvoid ]
+     PROP () RETURN () SEP (mem_mgr gv).*)
+
+(* Function-body correctness proofs *)
+*)
